experiments

proof/amd64/avx2/Keccak1600_avx2.ec
@@ -28,47 +28,7 @@ from CryptoSpecs require import FIPS202_SHA3 FIPS202_Keccakf1600.
 from CryptoSpecs require import Keccakf1600_Spec Keccak1600_Spec FIPS202_SHA3_Spec.
 *)
 
-(* circuit-friendly state mappings *)
-
-abbrev u256_bits64 (w: W256.t) k : W64.t =
- W64.init (fun i => w.[i+64*k]).
-
-lemma u256_bits64E w k:
- 0 <= k < 4 =>
- u256_bits64 w k = w \bits64 k.
-proof.
-move=> Hk; rewrite /u256_bits64.
-apply W64.ext_eq => i Hi.
-by rewrite bits64E initiE 1://= initiE 1://= /#.
-qed.
-
-op u256_pack4 (w0 w1 w2 w3: W64.t): W256.t =
- W256.init (fun i => if i < 64 then w0.[i]
-                     else if i < 128 then w1.[i-64]
-                     else if i < 192 then w2.[i-128]
-                     else w3.[i-192]).
-
-
-lemma u256_pack4E w0 w1 w2 w3:
- u256_pack4 w0 w1 w2 w3 = pack4 [w0; w1; w2; w3].
-proof.
-rewrite /u256_pack4; apply W256.ext_eq => k Hk.
-rewrite initiE 1:// pack4E initiE 1:// /=.
-rewrite get_of_list 1:/# /=.
-case: (k < 64) => C1.
- by rewrite ifT 1:/# modz_small /= /#.
-case: (k < 128) => C2.
- by rewrite ifF 1:/# ifT 1:/#; congr; smt().
-case: (k < 192) => C3.
- by rewrite ifF 1:/# ifF 1:/# ifT 1:/#; congr; smt().
-by rewrite ifF 1:/# ifF 1:/# ifF 1:/# ifT 1:/#; congr => /#.
-qed.
-
-lemma u256_pack4_zero:
- u256_pack4 W64.zero W64.zero W64.zero W64.zero = W256.zero.
-proof.
-by apply W256.all_eq_eq; rewrite /all_eq /u256_pack4 /=.
-qed.
+require import Avx2_extra.
 
 op stavx2_from_st25 (st: W64.t Array25.t): W256.t Array7.t =
  Array7.of_list W256.zero
@@ -118,11 +78,6 @@ move: {Hi} i; apply/List.allP => /=.
 by rewrite /stavx2_st0 /stavx2_from_st25 get_of_list 1:// /= /st0 !createiE 1..25:// u256_pack4_zero.
 qed.
 
-op u256_broadcastP w =
- u256_bits64 w 1 = u256_bits64 w 0
- /\ u256_bits64 w 2 = u256_bits64 w 0
- /\ u256_bits64 w 3 = u256_bits64 w 0.
-
 op stavx2INV (st: W256.t Array7.t): bool =
  u256_broadcastP st.[0].
 
@@ -153,22 +108,6 @@ proof.
 move=> H1 H2 E.
 by rewrite -(stavx2_to_st25K st1 _) 1:// -(stavx2_to_st25K st2 _) 1:// E.
 qed.
-
-lemma u256_broadcastP_VPBROADCAST w:
- u256_broadcastP (VPBROADCAST_4u64 w).
-proof.
-rewrite /VPBROADCAST_4u64 /u256_broadcastP.
-by rewrite !u256_bits64E 1..4:// !pack4bE 1..4:// /= -iotaredE /=.
-qed.
-
-lemma u256_broadcastP_xor w1 w2:
- u256_broadcastP w1 =>
- u256_broadcastP w2 =>
- u256_broadcastP (w1 `^` w2).
-proof.
-by rewrite /u256_broadcastP !u256_bits64E 1..12:// !xorb64E /#.
-qed.
-
 
 abbrev stF_avx2 f = fun st => stavx2_from_st25 (f (stavx2_to_st25 st)).
 
