proof/amd64/avx2/Keccak1600_avx2x4.ec
@@ -11,33 +11,16 @@ require import List Real Distr Int IntDiv CoreMap.
 
 from Jasmin require import JModel.
 
-from CryptoSpecs require import FIPS202_SHA3 FIPS202_Keccakf1600.
+from CryptoSpecs require import Bindings.
+from CryptoSpecs require export FIPS202_SHA3 FIPS202_Keccakf1600.
 from CryptoSpecs require import Keccakf1600_Spec Keccak1600_Spec FIPS202_SHA3_Spec.
 
 from JazzEC require import Jazz_avx2.
 
 
 from JazzEC require import WArray768 WArray200.
-from JazzEC require import Array24 Array5.
+from JazzEC require import Array25 Array24 Array5.
 
-
-(** lemmata (move?) *)
-lemma state2bytesE st i:
- (state2bytes st).[i] = (stbytes st).[i].
-proof.
-case: (0 <= i < 200) => C.
- admit.
-rewrite nth_out.
- by rewrite size_state2bytes.
-by rewrite get_out.
-qed.
-
-
-lemma bytes2state0: bytes2state [] = st0.
-admitted.
-
-lemma addstate_st0 st: addstate st0 st = st.
-admitted.
 
 require import StdOrder.
 import IntOrder.
@@ -52,7 +35,6 @@ move=> Hr8 Hi; rewrite /SQUEEZE1600 nth_take 1..2:/# /squeezeblocks.
 rewrite (BitEncoding.BitChunking.nth_flatten W8.zero r8).
  apply/List.allP => x /mapP [y [Hy ->]] /=.
  by rewrite size_squeezestate_i /#.
-search nth map.
 rewrite (nth_map 0).
  rewrite size_iota; split; first smt().
  move=> _; rewrite ltzE lez_maxr 1:/#.
@@ -65,7 +47,7 @@ move=> _; rewrite ltzE; smt(leq_div2r).
 qed.
 
 
-
+(*
 import Ring.IntID.
 
 lemma bits8_bits (w: W256.t) (k: int):
@@ -115,27 +97,231 @@ rewrite initiE //= unpack8E !initiE 1..2:/# /=; congr.
  congr; smt().
 smt().
 qed.
+*)
 
 
+require import Avx2_extra.
+
+import BitEncoding BitChunking.
+
+from JazzEC require import WArray800.
+
+op sliceget64_256_25 (arr: W256.t Array25.t) (offset: int) : W64.t = 
+ if 8 %| offset
+ then WArray800.get64_direct (WArray800.init256 (fun i => arr.[i])) (offset %/ 8)
+ else W64.bits2w (take 64 (drop offset (flatten (map W256.w2bits (to_list arr))))).
+
+bind op [W256.t & W64.t & Array25.t] sliceget64_256_25 "asliceget".
+realize bvaslicegetP.
+move => /= arr offset; rewrite /sliceget64_256_25 /= => H k kb. 
+case (8 %| offset) => /= *; last by smt(W64.get_bits2w).
+rewrite /get64_direct pack8E initiE 1:/# /= initiE 1:/# /= initiE 1:/# /= bits8E initiE 1:/# /=.
+rewrite nth_take 1,2:/# nth_drop 1,2:/#.
+rewrite (BitEncoding.BitChunking.nth_flatten false 256 _). 
+ by rewrite allP => x /=; rewrite mapP => He; elim He;smt(W256.size_w2bits).
+rewrite (nth_map W256.zero []); 1: smt(Array25.size_to_list).
+by rewrite nth_mkseq /#.
+qed.
+
+
+op sliceget256_64_25 (arr: W64.t Array25.t) (offset: int) : W256.t = 
+ if 8 %| offset
+ then  WArray200.get256_direct (WArray200.init64 (fun (i_0 : int) => arr.[i_0])) (offset %/ 8)
+ else W256.bits2w (take 256 (drop offset (flatten (map W64.w2bits (to_list arr))))).
+
+bind op [W64.t & W256.t & Array25.t] sliceget256_64_25 "asliceget".
+realize bvaslicegetP.
+move => /= arr offset; rewrite /sliceget256_64_25 /= => H k kb. 
+case (8 %| offset) => /= *; last by smt(W256.get_bits2w).
+rewrite /get256_direct pack32E initiE 1:/# /= initiE 1:/# /= initiE 1:/# /= bits8E initiE 1:/# /=.
+rewrite nth_take 1,2:/# nth_drop 1,2:/#.
+rewrite (BitEncoding.BitChunking.nth_flatten false 64 _). 
+ by rewrite allP => x /=; rewrite mapP => He; elim He;smt(W64.size_w2bits).
+rewrite (nth_map W64.zero []); 1: smt(Array25.size_to_list).
+by rewrite nth_mkseq /#.
+qed.
+
+op sliceset64_256_25 (arr: W256.t Array25.t) (offset: int) (bv: W64.t) : W256.t Array25.t =
+ if 8 %| offset
+ then Array25.init 
+       (fun i =>
+        WArray800.get256
+         (WArray800.set64_direct
+           (WArray800.init256 (fun j => arr.[j]))
+           (offset %/ 8)
+           bv)
+         i)
+ else Array25.of_list
+       witness
+       (map W256.bits2w
+            (chunk 256
+                   (take offset (flatten (map W256.w2bits (to_list arr)))
+                     ++ w2bits bv ++
+                     drop (offset+64) (flatten (map W256.w2bits (to_list arr)))))).
+
+lemma size_flatten_W256_w2bits (a : W256.t list) :
+  (size (flatten (map W256.w2bits (a))))  =  256 * size a.
+proof.
+rewrite (size_flatten' 256).
+ by move=> l /mapP [x [Hx ->]]; rewrite W256.size_w2bits.
+by rewrite size_map.
+qed.
+
+bind op [W256.t & W64.t & Array25.t] sliceset64_256_25 "asliceset".
+realize bvaslicesetP.
+move => arr offset bv H /= k kb; rewrite /sliceset64_256_25 /=.
+case (8 %| offset) => /= *; last first.
++ rewrite of_listK; 1: by rewrite size_map size_chunk 1:// !size_cat size_take;
+      by smt(size_take size_drop  W256.size_w2bits size_cat Array25.size_to_list size_flatten_W256_w2bits size_ge0). 
+  rewrite -(map_comp W256.w2bits W256.bits2w) /(\o). 
+  have := eq_in_map ((fun (x : bool list) => w2bits ((bits2w x))%W256)) idfun (chunk 256
+        (take offset (flatten (map W256.w2bits (to_list arr))) ++ w2bits bv ++
+         drop (offset + 64) (flatten (map W256.w2bits (to_list arr))))).
+  rewrite iffE => [#] -> * /=; 1: by smt(in_chunk_size W256.bits2wK).
+  rewrite map_id /= chunkK 1://;1: by rewrite !size_cat size_take;
+    by smt(size_take size_drop  W256.size_w2bits size_cat Array25.size_to_list size_flatten_W256_w2bits size_ge0). 
+  by rewrite !nth_cat !size_cat /=;
+     smt(nth_take nth_drop size_take size_drop  W256.size_w2bits size_cat Array25.size_to_list size_flatten_W256_w2bits size_ge0). 
+rewrite (nth_flatten _ 256); 1: by rewrite allP => i;rewrite mapP => He; elim He;smt(W256.size_w2bits).
+rewrite (nth_map W256.zero []); 1: smt(Array25.size_to_list).
+rewrite nth_mkseq 1:/# /= initiE 1:/# /= get256E pack32E initiE 1:/# /= initiE 1:/# /= /set64_direct.
+rewrite initiE 1:/# /=.
+case (offset <= k && k < offset + 64) => *; 1: by 
+  rewrite ifT 1:/#  get_bits8 /= 1,2:/# initiE // initiE //.
+rewrite ifF 1:/# initiE 1:/# /=.
+rewrite (nth_flatten _ 256); 1: by rewrite allP => i;rewrite mapP => He; elim He;smt(W256.size_w2bits).
+rewrite (nth_map W256.zero []); 1: smt(Array25.size_to_list).
+rewrite nth_mkseq 1:/# /= bits8E /= initiE /# /=.
+qed.
+
+op sliceset256_64_25 (arr: W64.t Array25.t) (offset: int) (bv: W256.t) : W64.t Array25.t =
+ if 8 %| offset
+ then Array25.init 
+       (fun i =>
+        WArray200.get64
+         (WArray200.set256_direct
+           (WArray200.init64 (fun j => arr.[j]))
+           (offset %/ 8)
+           bv)
+         i)
+ else Array25.of_list
+       witness
+       (map W64.bits2w
+            (chunk 64
+                   (take offset (flatten (map W64.w2bits (to_list arr)))
+                     ++ w2bits bv ++
+                     drop (offset+256) (flatten (map W64.w2bits (to_list arr)))))).
+
+lemma size_flatten_W64_w2bits (a : W64.t list) :
+  (size (flatten (map W64.w2bits (a))))  =  64 * size a.
+proof.
+rewrite (size_flatten' 64).
+ by move=> l /mapP [x [Hx ->]]; rewrite W64.size_w2bits.
+by rewrite size_map.
+qed.
+
+
+bind op [W64.t & W256.t & Array25.t] sliceset256_64_25 "asliceset".
+realize bvaslicesetP. 
+move => arr offset bv H /= k kb; rewrite /sliceset256_64_25 /=.
+case (8 %| offset) => /= *; last first.
++ rewrite of_listK; 1: by rewrite size_map size_chunk 1:// !size_cat size_take;
+      by smt(size_take size_drop  W64.size_w2bits size_cat Array25.size_to_list size_flatten_W64_w2bits size_ge0). 
+  rewrite -(map_comp W64.w2bits W64.bits2w) /(\o). 
+  have := eq_in_map ((fun (x : bool list) => w2bits ((bits2w x))%W64)) idfun (chunk 64
+        (take offset (flatten (map W64.w2bits (to_list arr))) ++ w2bits bv ++
+         drop (offset + 256) (flatten (map W64.w2bits (to_list arr))))).
+  rewrite iffE => [#] -> * /=; 1: by smt(in_chunk_size W64.bits2wK).
+  rewrite map_id /= chunkK 1://;1: by rewrite !size_cat size_take;
+    by smt(size_take size_drop  W64.size_w2bits size_cat Array25.size_to_list size_flatten_W64_w2bits size_ge0). 
+  by rewrite !nth_cat !size_cat /=;
+     smt(nth_take nth_drop size_take size_drop  W64.size_w2bits size_cat Array25.size_to_list size_flatten_W64_w2bits size_ge0). 
+rewrite (nth_flatten _ 64); 1: by rewrite allP => i;rewrite mapP => He; elim He;smt(W64.size_w2bits).
+rewrite (nth_map W64.zero []); 1: smt(Array25.size_to_list).
+rewrite nth_mkseq 1:/# /= initiE 1:/# /= get64E pack8E initiE 1:/# /= initiE 1:/# /= /set256_direct.
+rewrite initiE 1:/# /=.
+case (offset <= k && k < offset + 256) => *; 1: by 
+  rewrite ifT 1:/#  get_bits8 /= 1,2:/# initiE // initiE //.
+rewrite ifF 1:/# initiE 1:/# /=.
+rewrite (nth_flatten _ 64); 1: by rewrite allP => i;rewrite mapP => He; elim He;smt(W64.size_w2bits).
+rewrite (nth_map W64.zero []); 1: smt(Array25.size_to_list).
+rewrite nth_mkseq 1:/# /= bits8E /= initiE /# /=.
+qed.
 
 (** Packed 4x-state *)
+
 type state4x = W256.t Array25.t.
 
-op (\a25bits64) (a: state4x) (k: int): state =
- Array25.map (fun (x: W256.t) => W4u64.\bits64 x k) a.
+(*
+abbrev st4x_get (a: state4x) (k: int): state =
+ init_25_64 (fun i => u256_bits64 a.[i] k).
+*)
+abbrev st4x_get a k=
+ init_25_64 (fun i => sliceget64_256_25 a (8*(4*i+k)*8)).
 
-op (\a24bits64) (a: W256.t Array24.t) (k: int): W64.t Array24.t =
- Array24.map (fun (x: W256.t) => W4u64.\bits64 x k) a.
 
-op (\a5bits64) (a: W256.t Array5.t) (k: int): W64.t Array5.t =
- Array5.map (fun (x: W256.t) => W4u64.\bits64 x k) a.
+lemma st4x_getiE x k i:
+ 0 <= k < 4 =>
+ 0 <= i < 25 =>
+ (st4x_get x k).[i] = x.[i] \bits64 k.
+proof.  admit(*by move=> Hk Hi; rewrite initiE //= u256_bits64E*). qed.
 
-op a25pack4 (l: state list): state4x =
- Array25.init (fun i => pack4 (map (fun (s: state) => s.[i]) l)).
+abbrev st4x_pack (sts: state*state*state*state): state4x =
+ init_25_256 (fun i => u256_pack4 sts.`1.[i] sts.`2.[i] sts.`3.[i] sts.`4.[i]).
 
-op a25unpack4 (st4: state4x): state list =
- map (fun k=> st4 \a25bits64 k) (iota_ 0 4).
+lemma st4x_packiE (sts: state*state*state*state) i:
+ 0 <= i < 25 =>
+ (st4x_pack sts).[i] = u256_pack4 (sts.`1.[i]) (sts.`2.[i]) (sts.`3.[i]) (sts.`4.[i]).
+proof. by rewrite /st4x_pack => Hi; rewrite initiE //. qed.
 
+op st4x_unpack (st4: state4x): state*state*state*state =
+ ( st4x_get st4 0
+ , st4x_get st4 1
+ , st4x_get st4 2
+ , st4x_get st4 3
+ ).
+
+lemma st4x_unpackK st4x:
+ st4x_pack (st4x_unpack st4x) = st4x.
+proof.
+rewrite /st4x_pack /st4x_unpack.
+apply Array25.ext_eq => i Hi; rewrite initiE //.
+beta; iota.
+rewrite !st4x_getiE //=.
+rewrite u256_pack4E -{5}(unpack64K st4x.[i]); congr.
+by rewrite unpack64E init_of_list -iotaredE /=. 
+qed.
+
+lemma st4x_packK (sts: state*state*state*state):
+ st4x_unpack (st4x_pack sts) = sts.
+proof.
+move: sts => [st0 st1 st2 st3].
+rewrite /st4x_pack /st4x_unpack.
+congr; 
+ by (apply Array25.ext_eq => i Hi;
+     rewrite st4x_getiE //= initiE //= u256_pack4E pack4bE //).
+qed.
+
+abbrev st4x_map (f:W64.t Array25.t->W64.t Array25.t) (st4x:W256.t Array25.t): W256.t Array25.t =
+ st4x_pack (f (st4x_get st4x 0), f (st4x_get st4x 1), f (st4x_get st4x 2), f (st4x_get st4x 3)).
+
+lemma st4x_mapE (f: state->state) (st4x: state4x):
+ st4x_map f st4x
+ = st4x_pack (f (st4x_get st4x 0), f (st4x_get st4x 1), f (st4x_get st4x 2), f (st4x_get st4x 3)).
+proof.
+apply Array25.ext_eq => i Hi.
+by rewrite initiE //. 
+qed.
+
+(*op st4x_match (st4x: state4x) (st0 st1 st2 st3: state) =
+ st4x = st4x_pack (st0,st1,st2,st3).
+*)
+abbrev st4x_match st4x sts = (st4x = st4x_pack sts).
+
+
+
+
+(*
 lemma a25bits64iE x k i:
  0 <= i < 25 =>
  (x \a25bits64 k).[i] = x.[i] \bits64 k.
@@ -176,9 +362,6 @@ qed.
 
 op a5pack4 (l: (W64.t Array5.t) list): W256.t Array5.t =
  Array5.init (fun i => pack4 (map (fun (x: W64.t Array5.t) => x.[i]) l)).
-
-op match_state4x (st0 st1 st2 st3: state) (st4x: state4x) =
- st4x = a25pack4 [st0; st1; st2; st3].
 
 lemma a25pack4_eq stl st4x:
  a25pack4 stl = st4x
@@ -235,7 +418,7 @@ have: k \in iotared 0 4 by smt(mem_iota).
 by move: {Hk} k ; apply/List.allP.
 qed.
 
-
+*)
 (******************)
 
 
@@ -249,38 +432,38 @@ from JazzEC require import Array25 WArray200.
 
 
 
-op keccak_f1600_x4 = map_state4x keccak_f1600_op.
+op keccak_f1600_x4 = st4x_map keccak_f1600_op.
 
-op st0_avx2x4 = Array25.create W256.zero.
+op st4x0 = Array25.create W256.zero.
 
-op addstate_avx2x4 (st: W256.t Array25.t, l0 l1 l2 l3: W8.t list): W256.t Array25.t.
+lemma st4x0E: st4x_match st4x0 (st0,st0,st0,st0).
+proof.
+rewrite tP => i Hi.
+rewrite createiE // st4x_packiE //; iota.
+by rewrite !createiE // u256_pack4_zero.
+qed.
 
-lemma avx2x4_st0P:
- match_state4x st0 st0 st0 st0 st0_avx2x4.
-admitted.
 
+op addstate_avx2x4 (st: state4x, l0 l1 l2 l3: W8.t list): state4x.
 
-op absorb_spec_avx2x4 (r8: int) (tb: int) (l0 l1 l2 l3: W8.t list) stx4 =
- match_state4x
-  (ABSORB1600 (W8.of_int tb) r8 l0)
-  (ABSORB1600 (W8.of_int tb) r8 l1)
-  (ABSORB1600 (W8.of_int tb) r8 l2)
-  (ABSORB1600 (W8.of_int tb) r8 l3)
-  stx4.
+op absorb_spec_avx2x4 (r8: int) (tb: int) (l0 l1 l2 l3: W8.t list) st4x =
+ st4x_match st4x ( ABSORB1600 (W8.of_int tb) r8 l0
+                 , ABSORB1600 (W8.of_int tb) r8 l1
+                 , ABSORB1600 (W8.of_int tb) r8 l2
+                 , ABSORB1600 (W8.of_int tb) r8 l3).
 
-op pabsorb_spec_avx2x4 r8 l0 l1 l2 l3 stx4: bool =
+op pabsorb_spec_avx2x4 r8 l0 l1 l2 l3 st4x: bool =
  0 < r8 <= 200 /\
  size l1 = size l0 /\ size l2 = size l0 /\ size l3 = size l0 /\
- match_state4x
-  (addstate (stateabsorb_iblocks (chunk r8 l0) st0) (bytes2state (chunkremains r8 l0)))
-  (addstate (stateabsorb_iblocks (chunk r8 l1) st0) (bytes2state (chunkremains r8 l1)))
-  (addstate (stateabsorb_iblocks (chunk r8 l2) st0) (bytes2state (chunkremains r8 l2)))
-  (addstate (stateabsorb_iblocks (chunk r8 l3) st0) (bytes2state (chunkremains r8 l3)))
-  stx4.
+ st4x_match st4x
+            ( addstate (stateabsorb_iblocks (chunk r8 l0) st0) (bytes2state (chunkremains r8 l0))
+            , addstate (stateabsorb_iblocks (chunk r8 l1) st0) (bytes2state (chunkremains r8 l1))
+            , addstate (stateabsorb_iblocks (chunk r8 l2) st0) (bytes2state (chunkremains r8 l2))
+            , addstate (stateabsorb_iblocks (chunk r8 l3) st0) (bytes2state (chunkremains r8 l3))).
 
 lemma pabsorb_spec_avx2x4_nil r8:
  0 < r8 <= 200 =>
- pabsorb_spec_avx2x4 r8 [] [] [] [] st0_avx2x4.
+ pabsorb_spec_avx2x4 r8 [] [] [] [] st4x0.
 proof.
 admitted.
 
@@ -291,8 +474,10 @@ admitted.
 hoare state_init_avx2x4_h:
  Jazz_avx2.M.__state_init_avx2x4
  : true
- ==> match_state4x st0 st0 st0 st0 res.
-admitted.
+ ==> res = st4x0.
+proof.
+proc.
+admitted (* BDEP? *).
 
 
 lemma state_init_avx2x4_ll:
@@ -308,7 +493,7 @@ qed.
 phoare state_init_avx2x4_ph:
  [ Jazz_avx2.M.__state_init_avx2x4
  : true
- ==> match_state4x st0 st0 st0 st0 res
+ ==> res = st4x0
  ] = 1%r.
 admitted.
 
