proof/amd64/avx2/Keccakf1600_avx2x4.ec
@@ -1,15 +1,3 @@
-(******************************************************************************
-   Keccakf1600_avx2x4.ec:
-
-   Correctness proof for the 4x_AVX2 implementation
-
-
-   The 4x_AVX2 implementation is essentially a 4-way SIMD implementation of the
-  REF scalar implementation. The proof strategy is hence to prove equivalence
-  between any lane with REF, and deriving the parallel execution from generic
-  HL reasoning.
-
-******************************************************************************)
 require import List Real Distr Int IntDiv CoreMap.
 
 from Jasmin require import JModel.
@@ -17,13 +5,578 @@ from Jasmin require import JModel.
 from CryptoSpecs require import FIPS202_SHA3 FIPS202_Keccakf1600.
 from CryptoSpecs require import Keccakf1600_Spec.
 
-
 require import Keccakf1600_ref.
+require import Keccak1600_ref.
 require import Keccak1600_avx2x4.
 
 from JazzEC require Jazz_ref.
 from JazzEC require import Jazz_avx2.
 from JazzEC require import WArray768 Array5 Array25.
+
+from JazzEC require import WArray200 WArray800.
+from JazzEC require import Array100.
+
+
+op st4x_to_4st (st4x: state4x): state*state*state*state =
+ ( init_25_64 (fun i => sliceget64_256_25 st4x ((200*0+8*i)*8))
+ , init_25_64 (fun i => sliceget64_256_25 st4x ((200*1+8*i)*8))
+ , init_25_64 (fun i => sliceget64_256_25 st4x ((200*2+8*i)*8))
+ , init_25_64 (fun i => sliceget64_256_25 st4x ((200*3+8*i)*8))
+ ).
+
+
+bind array Array100."_.[_]" Array100."_.[_<-_]" Array100.to_list Array100.of_list Array100.t 100.
+realize tolistP by done.
+realize get_setP by smt(Array100.get_setE). 
+realize eqP by smt(Array100.tP).
+realize get_out by smt(Array100.get_out).
+
+op init_100_64 (f: int -> W64.t) = Array100.init f.
+
+bind op [W64.t & Array100.t] init_100_64 "ainit".
+realize bvainitP.
+proof.
+rewrite /init_100_64 => f.
+rewrite BVA_Top_Array100_Array100_t.tolistP.
+apply eq_in_mkseq => i i_bnd;
+smt(Array100.initE).
+qed.
+
+
+
+op sliceget256_64_100 (arr: W64.t Array100.t) (offset:int): W256.t =
+ if 8 %| offset
+ then WArray800.get256_direct
+       (WArray800.init64 (fun i => arr.[i]))
+       (offset %/ 8)
+ else W256.bits2w (take 256 (drop offset (flatten (map W64.w2bits (to_list arr))))).
+
+bind op [W64.t & W256.t & Array100.t] sliceget256_64_100 "asliceget".
+realize bvaslicegetP.
+move => /= arr offset; rewrite /sliceget256_64_100 /= => H k kb. 
+case (8 %| offset) => /= *; last by smt(W256.get_bits2w).
+rewrite /get256_direct pack32E initiE 1:/# /= initiE 1:/# /= initiE 1:/# /= bits8E initiE 1:/# /=.
+rewrite nth_take 1,2:/# nth_drop 1,2:/#.
+rewrite (BitEncoding.BitChunking.nth_flatten false 64 _). 
+ by rewrite allP => x /=; rewrite mapP => He; elim He;smt(W64.size_w2bits).
+rewrite (nth_map W64.zero []); 1: smt(Array100.size_to_list).
+by rewrite nth_mkseq /#.
+qed.
+
+
+abbrev st4x_from_4st (sts: state*state*state*state): state4x =
+ init_25_256
+  (fun i =>
+    sliceget256_64_100
+     (init_100_64
+      (fun j =>
+        if j < 25 then sts.`1.[j]
+        else if j < 50 then sts.`2.[j-25]
+        else if j < 75 then sts.`3.[j-50]
+        else sts.`4.[j-75]))
+      (32*i*8)
+    ).
+
+require import Avx2_extra.
+op st4x_pack_spec (sts: state4x): state4x =
+ st4x_pack (st4x_to_4st sts).
+
+op st4x_unpack_spec (st4x: state4x) =
+ st4x_from_4st (st4x_unpack st4x).
+(*
+  (init_25_64 (fun i => zero),init_25_64 (fun i => zero),init_25_64 (fun i => zero),init_25_64 (fun i => zero)). 
+*)
+op st4x_inv (_: state4x) = true.
+
+
+import BitEncoding BitChunking.
+lemma chunk1 ['a] n (l: 'a list):
+ size l = n =>
+ n <> 0 =>
+ chunk n l = [l].
+proof.
+rewrite /chunk.
+move=> Hn H0.
+by rewrite Hn divzz H0 b2i1 mkseq1 /= drop0 -Hn take_size.
+qed.
+
+lemma stx4_bvP (_a: state4x):
+ (map
+     (fun (temp : bool list) =>
+        (Array25.of_list W256.zero (map W256.bits2w (chunk 256 temp)))%Array7)
+     (chunk 6400 (flatten [flatten (map W256.w2bits (to_list _a))])))
+ = [_a].
+proof.
+rewrite flatten1 chunk_size 1://= /=.
+ rewrite (size_flatten_ctt 256).
+  by move=> bs /mapP => [[w [_ ->]]].
+ by rewrite size_map size_to_list.
+rewrite flattenK 1://.
+ move=> bs /mapP [l [Hl ->]].
+ by rewrite /w2bits size_mkseq.
+by rewrite -map_comp /(\o) /= map_id to_listK.
+qed.
+
+lemma X1 st4x:
+ Array25.of_list W256.zero
+  (map W256.bits2w (chunk 256 (flatten (map W256.w2bits (to_list st4x))))) = st4x.
+proof.
+rewrite tP => i Hi.
+rewrite get_of_list // (nth_map []).
+ rewrite size_chunk // (size_flatten' 256);
+   1: by  move=> l /mapP [y [Hy ->]]; smt(W256.size_w2bits).
+ by rewrite size_map size_to_list /#.
+rewrite flattenK //.
+ admit.
+rewrite (nth_map witness) //.
+by rewrite size_to_list.
+qed.
+
+lemma X2 (st0 st1 st2 st3:state):
+ WArray800.init256
+  (fun (i : int) =>
+   (Array25.of_list W256.zero
+           (map W256.bits2w
+              (chunk 256
+                 (flatten (map W64.w2bits (to_list st0)) ++
+                  (flatten (map W64.w2bits (to_list st1)) ++
+                   (flatten (map W64.w2bits (to_list st2)) ++
+                    flatten (map W64.w2bits (to_list st3)))))))).[i])
+ = WArray800.init64
+    (fun i => (Array100.of_list W64.zero (to_list st0++to_list st1++to_list st2++to_list st3)).[i]).
+proof.
+admitted.
+
+lemma X3 (x: W64.t Array100.t) i:
+ 0 <= i < 100 =>
+ get64
+  (WArray800.init64
+     (fun (i0 : int) => x.[i0])) i
+ = x.[i].
+proof.
+move=> Hi.
+search WArray800.init64.
+search WArray800.get64_direct.
+rewrite get64E pack8E.
+apply W64.ext_eq => k Hk.
+rewrite initiE //= initiE 1:/# /= initiE 1:/# /=.
+rewrite bits8iE 1:/# /#.
+qed.
+
+lemma XX (st0 st1 st2 st3:state) i:
+ 0 <= i < 100 =>
+ get64
+  (WArray800.init256
+     (fun (i0 : int) =>
+        (Array25.of_list W256.zero
+           (map W256.bits2w
+              (chunk 256
+                 (flatten (map W64.w2bits (to_list st0)) ++
+                  (flatten (map W64.w2bits (to_list st1)) ++
+                   (flatten (map W64.w2bits (to_list st2)) ++
+                    flatten (map W64.w2bits (to_list st3)))))))).[i0])) i
+ = if i < 25
+   then st0.[i]
+   else if i < 50
+        then st1.[i-25]
+        else if i < 75
+             then st2.[i-50]
+             else st3.[i-75].
+proof.
+move=> Hi; rewrite X2 X3 // get_of_list // -!catA.
+case: (i<25) => C1.
+ rewrite nth_cat !size_to_list ifT 1:/#.
+ rewrite -get_to_list.
+ apply nth_change_dfl.
+ by rewrite size_to_list /#.
+case: (i<50) => C2.
+ rewrite nth_cat !size_to_list ifF 1:/#.
+ rewrite nth_cat !size_to_list ifT 1:/#.
+ rewrite -get_to_list.
+ apply nth_change_dfl.
+ by rewrite size_to_list /#.
+case: (i<75) => C3.
+ rewrite nth_cat !size_to_list ifF 1:/#.
+ rewrite nth_cat !size_to_list ifF 1:/#.
+ rewrite nth_cat !size_to_list ifT 1:/#.
+ rewrite -get_to_list.
+ apply nth_change_dfl.
+ by rewrite size_to_list /#.
+rewrite nth_cat !size_to_list ifF 1:/#.
+rewrite nth_cat !size_to_list ifF 1:/#.
+rewrite nth_cat !size_to_list ifF 1:/#.
+rewrite -get_to_list.
+apply nth_change_dfl.
+by rewrite size_to_list /#.
+qed.
+
+
+
+hoare st4x_pack_h _st0 _st1 _st2 _st3:
+ Jazz_avx2.M.__st4x_pack:
+ st0 = _st0 /\ st1 = _st1 /\ st2 = _st2 /\ st3 = _st3
+ ==> res = st4x_pack (_st0, _st1, _st2, _st3).
+proof.
+proc.
+proc change ^while.1: (sliceget256_64_25 st0 (32*i*8));
+ 1: by auto => /#.
+proc change ^while.2: (sliceget256_64_25 st1 (32*i*8));
+ 1: by auto => /#.
+proc change ^while.3: (sliceget256_64_25 st2 (32*i*8));
+ 1: by auto => /#.
+proc change ^while.4: (sliceget256_64_25 st3 (32*i*8));
+ 1: by auto => /#.
+unroll for 2.
+proc change 60: (sliceset64_256_25 st4x (8*(4 * 24 + 0)*8) t0);
+ 1: by auto => /#.
+proc change 61: (sliceset64_256_25 st4x (8*(4 * 24 + 1)*8) t1);
+ 1: by auto => /#.
+proc change 62: (sliceset64_256_25 st4x (8*(4 * 24 + 2)*8) t2);
+ 1: by auto => /#.
+proc change 63: (sliceset64_256_25 st4x (8*(4 * 24 + 3)*8) t3);
+ 1: by auto => /#.
+inline*; simplify.
+swap 127 8; wp 134.
+bdep 6400 6400
+     [_st0;_st1;_st2;_st3] [st0;st1;st2;st3] [st4x]
+     st4x_pack_spec
+     st4x_inv.
++ by move=> &m /> *; rewrite all_predT.
+move=> &m /> st4x /=.
+rewrite /st4x_pack_spec !flatten_cons flatten_nil !cats0.
+rewrite chunk1 //.
+ rewrite !size_cat !(size_flatten' 64);
+  1..4: by  move=> l /mapP [y [Hy ->]]; smt(W64.size_w2bits).
+ by rewrite !size_map !size_iota /#.
+rewrite chunk1 //.
+ rewrite (size_flatten' 256);
+  1: by  move=> l /mapP [y [Hy ->]]; smt(W256.size_w2bits).
+ by rewrite !size_map !size_iota /#.
+rewrite /= X1 => <-.
+rewrite tP => i Hi.
+rewrite !initiE //= /st4x_to_4st /=; congr.
++ rewrite !initiE //= /sliceget64_256_25 ifT 1:/#.
+  rewrite (:8*i*8 %/ 8=8*i) 1:/# XX /#.
++ rewrite !initiE //= /sliceget64_256_25 ifT 1:/#.
+  rewrite (:(200+8*i)*8 %/ 8=8*(25+i)) 1:/# XX /#.
++ rewrite !initiE //= /sliceget64_256_25 ifT 1:/#.
+  rewrite (:(400+8*i)*8 %/ 8=8*(50+i)) 1:/# XX /#.
++ rewrite !initiE //= /sliceget64_256_25 ifT 1:/#.
+  rewrite (:(600+8*i)*8 %/ 8=8*(75+i)) 1:/# XX /#.
+qed.
+
+
+hoare st4x_unpack_h _st4x:
+ Jazz_avx2.M.__st4x_unpack:
+ st4x = _st4x
+ ==> res = st4x_unpack _st4x.
+proof.
+proc; simplify.
+proc change ^while.6: (sliceset256_64_25 st0 (4*8*i*8) x0);
+ 1: by auto => /#.
+proc change ^while.7: (sliceset256_64_25 st1 (4*8*i*8) x1);
+ 1: by auto => /#.
+proc change ^while.8: (sliceset256_64_25 st2 (4*8*i*8) x2);
+ 1: by auto => /#.
+proc change ^while.9: (sliceset256_64_25 st3 (4*8*i*8) x3);
+ 1: by auto => /#.
+proc change 3: (sliceget64_256_25 st4x (8*(4*24)*8));
+ 1: by auto => /#.
+proc change 4: (sliceget64_256_25 st4x (8*(4*24+1)*8));
+ 1: by auto => /#.
+proc change 5: (sliceget64_256_25 st4x (8*(4*24+2)*8));
+ 1: by auto => /#.
+proc change 6: (sliceget64_256_25 st4x (8*(4*24+3)*8));
+ 1: by auto => /#.
+unroll for 2.
+swap 55 8.
+wp 62.
+inline*.
+bdep 6400 6400
+     [_st4x] [st4x] [st0;st1;st2;st3]
+     st4x_unpack_spec
+     st4x_inv.
++ by move=> &m /> *; rewrite all_predT.
+move=> &m /> st0 st1 st2 st3 /=.
+rewrite /st4x_unpack_spec !flatten_cons flatten_nil !cats0.
+rewrite chunk1 //=. admit.
+rewrite chunk1 //=. admit.
+rewrite chunk1 //=. admit.
+admitted.
+
+op st4x_id (x:state4x) = x.
+op st4x_id2 (x:state4x) = st4x_from_4st (st4x_to_4st x).
+
+op st_inv (_:state) = true.
+
+module MM = {
+ proc ttt1(st4x: state4x): state4x = {
+  var st0, st1, st2, st3: state;
+  (st0, st1, st2, st3) <@ M.__st4x_unpack(st0, st1, st2, st3, st4x);
+  st4x <@ M.__st4x_pack(st4x, st0, st1, st2, st3);
+  return st4x;
+  }
+ proc ttt2(st0 st1 st2 st3: state): state*state*state*state = {
+  var st4x: state4x;
+  st4x <@ M.__st4x_pack(st4x, st0, st1, st2, st3);
+  (st0, st1, st2, st3) <@ M.__st4x_unpack(st0, st1, st2, st3, st4x);
+  return (st0,st1,st2,st3);
+  }
+}.
+
+hoare test1 _st4x:
+ MM.ttt1:
+ st4x = _st4x
+ ==> res = _st4x.
+proof.
+proc; inline*.
+proc change ^while.18: (sliceset256_64_25 st00 (4*8*i*8) x0);
+ 1: by auto => /#.
+proc change ^while.19: (sliceset256_64_25 st10 (4*8*i*8) x1);
+ 1: by auto => /#.
+proc change ^while.20: (sliceset256_64_25 st20 (4*8*i*8) x2);
+ 1: by auto => /#.
+proc change ^while.21: (sliceset256_64_25 st30 (4*8*i*8) x3);
+ 1: by auto => /#.
+proc change 8: (sliceget64_256_25 st4x0 (8*(4*24)*8));
+ 1: by auto => /#.
+proc change 9: (sliceget64_256_25 st4x0 (8*(4*24+1)*8));
+ 1: by auto => /#.
+proc change 10: (sliceget64_256_25 st4x0 (8*(4*24+2)*8));
+ 1: by auto => /#.
+proc change 11: (sliceget64_256_25 st4x0 (8*(4*24+3)*8));
+ 1: by auto => /#.
+unroll for 7.
+swap 132 25.
+proc change ^while.1: (sliceget256_64_25 st01 (32*i0*8));
+ 1: by auto => /#.
+proc change ^while.2: (sliceget256_64_25 st11 (32*i0*8));
+ 1: by auto => /#.
+proc change ^while.3: (sliceget256_64_25 st21 (32*i0*8));
+ 1: by auto => /#.
+proc change ^while.4: (sliceget256_64_25 st31 (32*i0*8));
+ 1: by auto => /#.
+proc change 152: (sliceset64_256_25 st4x1 (8*(4 * 24 + 0)*8) t00);
+ 1: by auto => /#.
+proc change 153: (sliceset64_256_25 st4x1 (8*(4 * 24 + 1)*8) t10);
+ 1: by auto => /#.
+proc change 154: (sliceset64_256_25 st4x1 (8*(4 * 24 + 2)*8) t20);
+ 1: by auto => /#.
+proc change 155: (sliceset64_256_25 st4x1 (8*(4 * 24 + 3)*8) t30);
+ 1: by auto => /#.
+unroll for 147.
+swap 272 9; wp 280.
+bdep 6400 6400
+     [_st4x] [st4x] [st4x]
+     st4x_id2
+     st4x_inv.
+admitted.
+
+hoare test2 _st0 _st1 _st2 _st3:
+ MM.ttt2:
+ st0 = _st0 /\ st1 = _st1 /\ st2 = _st2 /\ st3 = _st3 
+ ==> res.`1 = _st0
+     /\ res.`2 = _st1
+     /\ res.`3 = _st2
+     /\ res.`4 = _st3.
+proof.
+proc; inline*; simplify.
+proc change ^while.1: (sliceget256_64_25 st00 (32*i*8));
+ 1: by auto => /#.
+proc change ^while.2: (sliceget256_64_25 st10 (32*i*8));
+ 1: by auto => /#.
+proc change ^while.3: (sliceget256_64_25 st20 (32*i*8));
+ 1: by auto => /#.
+proc change ^while.4: (sliceget256_64_25 st30 (32*i*8));
+ 1: by auto => /#.
+proc change 12: (sliceset64_256_25 st4x0 (8*(4 * 24 + 0)*8) t0);
+ 1: by auto => /#.
+proc change 13: (sliceset64_256_25 st4x0 (8*(4 * 24 + 1)*8) t1);
+ 1: by auto => /#.
+proc change 14: (sliceset64_256_25 st4x0 (8*(4 * 24 + 2)*8) t2);
+ 1: by auto => /#.
+proc change 15: (sliceset64_256_25 st4x0 (8*(4 * 24 + 3)*8) t3);
+ 1: by auto => /#.
+unroll for 7.
+swap 132 25.
+proc change ^while.18: (sliceset256_64_25 st01 (4*8*i0*8) x00);
+ 1: by auto => /#.
+proc change ^while.19: (sliceset256_64_25 st11 (4*8*i0*8) x10);
+ 1: by auto => /#.
+proc change ^while.20: (sliceset256_64_25 st21 (4*8*i0*8) x20);
+ 1: by auto => /#.
+proc change ^while.21: (sliceset256_64_25 st31 (4*8*i0*8) x30);
+ 1: by auto => /#.
+proc change 148: (sliceget64_256_25 st4x1 (8*(4*24)*8));
+ 1: by auto => /#.
+proc change 149: (sliceget64_256_25 st4x1 (8*(4*24+1)*8));
+ 1: by auto => /#.
+proc change 150: (sliceget64_256_25 st4x1 (8*(4*24+2)*8));
+ 1: by auto => /#.
+proc change 151: (sliceget64_256_25 st4x1 (8*(4*24+3)*8));
+ 1: by auto => /#.
+unroll for 147.
+swap 272 9; wp 280.
+bdep 6400 6400
+     [_st0;_st1;_st2;_st3] [st0;st1;st2;st3] [st0;st1;st2;st3]
+     st4x_id
+     st4x_inv.
+admitted.
+
+hoare keccak_pround_avx2x4_h _st0 _st1 _st2 _st3:
+ Jazz_avx2.M.__keccakf1600_pround_unpacked:
+ st0 = _st0 /\ st1 = _st1 /\ st2 = _st2 /\ st3 = _st3
+ ==> res.`1 = keccak_pround_op _st0
+     /\ res.`2 = keccak_pround_op _st1
+     /\ res.`3 = keccak_pround_op _st2
+     /\ res.`4 = keccak_pround_op _st3.
+proof.
+proc; simplify.
+inline __st4x_pack.
+proc change ^while.1: (sliceget256_64_25 st00 (32*i*8));
+ 1: by auto => /#.
+proc change ^while.2: (sliceget256_64_25 st10 (32*i*8));
+ 1: by auto => /#.
+proc change ^while.3: (sliceget256_64_25 st20 (32*i*8));
+ 1: by auto => /#.
+proc change ^while.4: (sliceget256_64_25 st30 (32*i*8));
+ 1: by auto => /#.
+proc change 16: (sliceset64_256_25 st4x (8*(4 * 24 + 0)*8) t0);
+ 1: by auto => /#.
+proc change 17: (sliceset64_256_25 st4x (8*(4 * 24 + 1)*8) t1);
+ 1: by auto => /#.
+proc change 18: (sliceset64_256_25 st4x (8*(4 * 24 + 2)*8) t2);
+ 1: by auto => /#.
+proc change 19: (sliceset64_256_25 st4x (8*(4 * 24 + 3)*8) t3);
+ 1: by auto => /#.
+unroll for 11.
+swap 64 11; wp 74.
+inline __st4x_unpack.
+proc change ^while.6: (sliceset256_64_25 st01 (4*8*i0*8) x00);
+ 1: by auto => /#.
+proc change ^while.7: (sliceset256_64_25 st11 (4*8*i0*8) x10);
+ 1: by auto => /#.
+proc change ^while.8: (sliceset256_64_25 st21 (4*8*i0*8) x20);
+ 1: by auto => /#.
+proc change ^while.9: (sliceset256_64_25 st31 (4*8*i0*8) x30);
+ 1: by auto => /#.
+proc change 81: (sliceget64_256_25 st4x0 (8*(4*24)*8));
+ 1: by auto => /#.
+proc change 82: (sliceget64_256_25 st4x0 (8*(4*24+1)*8));
+ 1: by auto => /#.
+proc change 83: (sliceget64_256_25 st4x0 (8*(4*24+2)*8));
+ 1: by auto => /#.
+proc change 84: (sliceget64_256_25 st4x0 (8*(4*24+3)*8));
+ 1: by auto => /#.
+unroll for 80.
+swap 133 9; wp 141.
+inline*.
+admit(*
+bdep 1600 1600
+     [_st0;_st1;_st2;_st3] [st0;st1;st2;st3] [st0;st1;st2;st3]
+     keccak_pround_op
+     st_inv.
+*).
+qed.
+
+print st4x_map.
+print st4x_get.
+
+op st4x_keccak_pround =
+ st4x_map keccak_pround_op.
+
+hoare keccak_pround_avx2x4_h2 _st4x:
+ Jazz_avx2.M.__keccakf1600_4x_pround:
+ a_357 = _st4x
+ ==> res = st4x_keccak_pround _st4x.
+proof.
+proc; simplify.
+(*
+(* não consegue lidar com isto... (grande demais?)*)
+bdep 6400 6400
+ [_st4x] [a_357] [e_356]
+ st4x_keccak_pround st4x_inv.
+*)
+admitted.
+
+
+
+
+
+from CryptoSpecs require import FIPS202_Keccakf1600.
+print state.
+
+op st00 = init_25_64 (fun _ => W64.zero).
+require import Avx2_extra.
+op st4x_keccak_pround2 (x:state4x) = 
+ init_25_256 (fun _ => u256_pack4 W64.zero W64.zero W64.zero W64.zero).
+op st4x_keccak_pround3 (x:state4x) = 
+ init_25_256 (fun i => u256_pack4 st00.[i] st00.[i] st00.[i] st00.[i]).
+print st4x_map.
+print st4x_get.
+print u256_bits64.
+
+op srl_256 (w1 w2 : W256.t) : W256.t =
+w1 `>>>` to_uint w2.
+
+bind op [W256.t] srl_256 "shr".
+realize bvshrP.
+rewrite /shr_256 => bv1 bv2.
+by rewrite W256.to_uint_shr; 1:smt(W256.to_uint_cmp).
+qed.
+
+op sliceget256_64 (a: W256.t) (offset: int) : W64.t =
+W4u64.truncateu64 (srl_256 a (W256.of_int offset)).
+
+abbrev u256_bits64' (w : W256.t) (k : int) : W64.t =
+sliceget256_64 w (k*64).
+
+print st4x_get.
+abbrev st4x_get' (a : state4x) (k : int) : FIPS202_Keccakf1600.state =
+  init_25_64 (fun (i : int) => u256_bits64 a.[i] k).
+print st4x_map.
+abbrev st4x_map2 (f : W64.t Array25.t -> W64.t Array25.t)
+  (st4x : W256.t Array25.t) : W256.t Array25.t =
+  st4x_pack
+    (f (st4x_get' st4x 0), f (st4x_get' st4x 1), f (st4x_get' st4x 2),
+     f (st4x_get' st4x 3)).
+
+(*
+abbrev st4x_pack (sts : state * state *
+  state * state) : state4x =
+  init_25_256
+    (fun (i : int) => u256_pack4 sts.`1.[i] sts.`2.[i] sts.`3.[i] sts.`4.[i]).
+*)
+op st4x_keccak_pround4 (x:state4x) = 
+ st4x_pack (st4x_get x 0, st4x_get x 0, st4x_get x 0, st4x_get x 0).
+op st4x_keccak_pround5 (x:state4x) = 
+ st4x_pack (st0,st0,st0,st0).
+
+print keccak_pround_op.
+
+op X_op (x:W64.t Array25.t)= x.
+op X0 = st4x_map2 X_op.
+op X1 = st4x_map2 keccak_theta_op.
+print st4x_pack.
+print st4x_map.
+
+hoare keccak_pround_avx2x4_h _a:
+ Jazz_avx2_inlined.M._keccakf1600_4x_pround :
+ a = _a /\ r8 = rOL8 /\ r56 = rOL56
+ ==> res = st4x_keccak_pround2 _a.
+proof.
+proc.
+simplify.
+bdep 6400 6400 [_a] [a] [e] st4x_keccak_pround st4x_inv.
+print st4x_keccak_pround.
+bdep 6400 6400 [_a] [a] [a] X1 st4x_inv.
++ rewrite allP => />.
++ move=> />.
+  by rewrite stavx2x4_bvP /stavx2x4_keccak_pround /= => ->.
+qed.
+
+
+(*op stavx2x4_keccak_pround = stF_avx2 keccak_pround_op.*)
 
 
 (** lemmata (move?) *)
