proof/amd64/avx2/Avx2_extra.ec
@@ -1,0 +1,76 @@
+require import AllCore List IntDiv.
+from Jasmin require import JWord JUtils.
+
+from CryptoSpecs require import Bindings.
+
+(* circuit-friendly state mappings *)
+
+abbrev u256_bits64 (w: W256.t) k : W64.t =
+ W64.init (fun i => w.[i+64*k]).
+
+lemma u256_bits64E w k:
+ 0 <= k < 4 =>
+ u256_bits64 w k = w \bits64 k.
+proof.
+move=> Hk; rewrite /u256_bits64.
+apply W64.ext_eq => i Hi.
+by rewrite bits64E initiE 1://= initiE 1://= /#.
+qed.
+
+
+op u256_pack4 (w0 w1 w2 w3 : W64.t) : W256.t =
+ concat_2u128 (concat_2u64 w0 w1) (concat_2u64 w2 w3).
+(*
+op u256_pack4 (w0 w1 w2 w3: W64.t): W256.t =
+ W256.init (fun i => if i < 64 then w0.[i]
+                     else if i < 128 then w1.[i-64]
+                     else if i < 192 then w2.[i-128]
+                     else w3.[i-192]).
+*)
+
+lemma u256_pack4E w0 w1 w2 w3:
+ u256_pack4 w0 w1 w2 w3 = pack4 [w0; w1; w2; w3].
+proof.
+admitted(*
+rewrite /u256_pack4; apply W256.ext_eq => k Hk.
+rewrite initiE 1:// pack4E initiE 1:// /=.
+rewrite get_of_list 1:/# /=.
+case: (k < 64) => C1.
+ by rewrite ifT 1:/# modz_small /= /#.
+case: (k < 128) => C2.
+ by rewrite ifF 1:/# ifT 1:/#; congr; smt().
+case: (k < 192) => C3.
+ by rewrite ifF 1:/# ifF 1:/# ifT 1:/#; congr; smt().
+by rewrite ifF 1:/# ifF 1:/# ifF 1:/# ifT 1:/#; congr => /#.
+qed.
+*).
+
+lemma u256_pack4_zero:
+ u256_pack4 W64.zero W64.zero W64.zero W64.zero = W256.zero.
+proof.
+admitted(*
+by apply W256.all_eq_eq; rewrite /all_eq /u256_pack4 /=.
+qed.
+*).
+
+op u256_broadcastP w =
+ u256_bits64 w 1 = u256_bits64 w 0
+ /\ u256_bits64 w 2 = u256_bits64 w 0
+ /\ u256_bits64 w 3 = u256_bits64 w 0.
+
+lemma u256_broadcastP_VPBROADCAST w:
+ u256_broadcastP (VPBROADCAST_4u64 w).
+proof.
+rewrite /VPBROADCAST_4u64 /u256_broadcastP.
+by rewrite !u256_bits64E 1..4:// !pack4bE 1..4:// /= -iotaredE /=.
+qed.
+
+lemma u256_broadcastP_xor w1 w2:
+ u256_broadcastP w1 =>
+ u256_broadcastP w2 =>
+ u256_broadcastP (w1 `^` w2).
+proof.
+by rewrite /u256_broadcastP !u256_bits64E 1..12:// !xorb64E /#.
+qed.
+
+
