proof/amd64/extracted/Jazz_ref.ec
@@ -257,23 +257,19 @@ module M = {
       tRAIL <- 0;
     } else {
       if ((8 <= lEN)) {
-        w <- (loadW64 Glob.mem (W64.to_uint (buf + (W64.of_int 0))));
+        w <- (loadW64 Glob.mem (W64.to_uint buf));
         buf <- (buf + (W64.of_int 8));
         lEN <- (lEN - 8);
       } else {
         if ((4 <= lEN)) {
-          w <-
-          (zeroextu64 (loadW32 Glob.mem (W64.to_uint (buf + (W64.of_int 0))))
-          );
+          w <- (zeroextu64 (loadW32 Glob.mem (W64.to_uint buf)));
           buf <- (buf + (W64.of_int 4));
           lEN <- (lEN - 4);
         } else {
           w <- (W64.of_int 0);
         }
         if ((2 <= lEN)) {
-          t16 <-
-          (zeroextu64 (loadW16 Glob.mem (W64.to_uint (buf + (W64.of_int 0))))
-          );
+          t16 <- (zeroextu64 (loadW16 Glob.mem (W64.to_uint buf)));
           buf <- (buf + (W64.of_int 2));
           lEN <- (lEN - 2);
         } else {
@@ -281,9 +277,7 @@ module M = {
         }
         if (((1 <= lEN) \/ ((tRAIL %% 256) <> 0))) {
           if ((1 <= lEN)) {
-            t8 <-
-            (zeroextu64
-            (loadW8 Glob.mem (W64.to_uint (buf + (W64.of_int 0)))));
+            t8 <- (zeroextu64 (loadW8 Glob.mem (W64.to_uint buf)));
             if (((tRAIL %% 256) <> 0)) {
               t8 <- (t8 `|` (W64.of_int (256 * (tRAIL %% 256))));
             } else {
@@ -315,9 +309,7 @@ module M = {
       w <- (set0_256);
     } else {
       if ((8 <= lEN)) {
-        w <-
-        (VPBROADCAST_4u64
-        (loadW64 Glob.mem (W64.to_uint (buf + (W64.of_int 0)))));
+        w <- (VPBROADCAST_4u64 (loadW64 Glob.mem (W64.to_uint buf)));
         buf <- (buf + (W64.of_int 8));
         lEN <- (lEN - 8);
       } else {
@@ -336,13 +328,12 @@ module M = {
       w <- (set0_128);
     } else {
       if ((16 <= lEN)) {
-        w <- (loadW128 Glob.mem (W64.to_uint (buf + (W64.of_int 0))));
+        w <- (loadW128 Glob.mem (W64.to_uint buf));
         buf <- (buf + (W64.of_int 16));
         lEN <- (lEN - 16);
       } else {
         if ((8 <= lEN)) {
-          w <-
-          (VMOV_64 (loadW64 Glob.mem (W64.to_uint (buf + (W64.of_int 0)))));
+          w <- (VMOV_64 (loadW64 Glob.mem (W64.to_uint buf)));
           buf <- (buf + (W64.of_int 8));
           lEN <- (lEN - 8);
           (buf, lEN, tRAIL, t64) <@ __mread_subu64 (buf, lEN, tRAIL);
@@ -364,12 +355,12 @@ module M = {
       w <- (set0_256);
     } else {
       if ((32 <= lEN)) {
-        w <- (loadW256 Glob.mem (W64.to_uint (buf + (W64.of_int 0))));
+        w <- (loadW256 Glob.mem (W64.to_uint buf));
         buf <- (buf + (W64.of_int 32));
         lEN <- (lEN - 32);
       } else {
         if ((16 <= lEN)) {
-          t128_0 <- (loadW128 Glob.mem (W64.to_uint (buf + (W64.of_int 0))));
+          t128_0 <- (loadW128 Glob.mem (W64.to_uint buf));
           buf <- (buf + (W64.of_int 16));
           lEN <- (lEN - 16);
           (buf, lEN, tRAIL, t128_1) <@ __mread_subu128 (buf, lEN, tRAIL);
@@ -393,15 +384,12 @@ module M = {
     
     if ((0 < lEN)) {
       if ((8 <= lEN)) {
-        Glob.mem <-
-        (storeW64 Glob.mem (W64.to_uint (buf + (W64.of_int 0))) w);
+        Glob.mem <- (storeW64 Glob.mem (W64.to_uint buf) w);
         buf <- (buf + (W64.of_int 8));
         lEN <- (lEN - 8);
       } else {
         if ((4 <= lEN)) {
-          Glob.mem <-
-          (storeW32 Glob.mem (W64.to_uint (buf + (W64.of_int 0)))
-          (truncateu32 w));
+          Glob.mem <- (storeW32 Glob.mem (W64.to_uint buf) (truncateu32 w));
           w <- (w `>>` (W8.of_int 32));
           buf <- (buf + (W64.of_int 4));
           lEN <- (lEN - 4);
@@ -409,9 +397,7 @@ module M = {
           
         }
         if ((2 <= lEN)) {
-          Glob.mem <-
-          (storeW16 Glob.mem (W64.to_uint (buf + (W64.of_int 0)))
-          (truncateu16 w));
+          Glob.mem <- (storeW16 Glob.mem (W64.to_uint buf) (truncateu16 w));
           w <- (w `>>` (W8.of_int 16));
           buf <- (buf + (W64.of_int 2));
           lEN <- (lEN - 2);
@@ -419,9 +405,7 @@ module M = {
           
         }
         if ((1 <= lEN)) {
-          Glob.mem <-
-          (storeW8 Glob.mem (W64.to_uint (buf + (W64.of_int 0)))
-          (truncateu8 w));
+          Glob.mem <- (storeW8 Glob.mem (W64.to_uint buf) (truncateu8 w));
           buf <- (buf + (W64.of_int 1));
           lEN <- (lEN - 1);
         } else {
@@ -437,15 +421,13 @@ module M = {
     var t64:W64.t;
     if ((0 < lEN)) {
       if ((16 <= lEN)) {
-        Glob.mem <-
-        (storeW128 Glob.mem (W64.to_uint (buf + (W64.of_int 0))) w);
+        Glob.mem <- (storeW128 Glob.mem (W64.to_uint buf) w);
         buf <- (buf + (W64.of_int 16));
         lEN <- (lEN - 16);
       } else {
         if ((8 <= lEN)) {
           Glob.mem <-
-          (storeW64 Glob.mem (W64.to_uint (buf + (W64.of_int 0)))
-          (MOVV_64 (truncateu64 w)));
+          (storeW64 Glob.mem (W64.to_uint buf) (MOVV_64 (truncateu64 w)));
           buf <- (buf + (W64.of_int 8));
           lEN <- (lEN - 8);
           w <- (VPUNPCKH_2u64 w w);
@@ -464,15 +446,13 @@ module M = {
     var t128:W128.t;
     if ((0 < lEN)) {
       if ((32 <= lEN)) {
-        Glob.mem <-
-        (storeW256 Glob.mem (W64.to_uint (buf + (W64.of_int 0))) w);
+        Glob.mem <- (storeW256 Glob.mem (W64.to_uint buf) w);
         buf <- (buf + (W64.of_int 32));
         lEN <- (lEN - 32);
       } else {
         t128 <- (truncateu128 w);
         if ((16 <= lEN)) {
-          Glob.mem <-
-          (storeW128 Glob.mem (W64.to_uint (buf + (W64.of_int 0))) t128);
+          Glob.mem <- (storeW128 Glob.mem (W64.to_uint buf) t128);
           buf <- (buf + (W64.of_int 16));
           lEN <- (lEN - 16);
           t128 <- (VEXTRACTI128 w (W8.of_int 1));
@@ -518,7 +498,7 @@ module M = {
         tRAILB <- 0;
       } else {
         if ((8 <= lEN)) {
-          t <- (loadW64 Glob.mem (W64.to_uint (buf + (W64.of_int 0))));
+          t <- (loadW64 Glob.mem (W64.to_uint buf));
           buf <- (buf + (W64.of_int (8 - lO)));
         } else {
           (buf,  _0,  _1, t) <@ __mread_subu64 (buf, (8 - lO), tRAILB);
@@ -535,7 +515,7 @@ module M = {
     }
     if ((8 <= lEN)) {
       while ((at \ult (W64.of_int ((aT %/ 8) + (lEN %/ 8))))) {
-        t <- (loadW64 Glob.mem (W64.to_uint (buf + (W64.of_int 0))));
+        t <- (loadW64 Glob.mem (W64.to_uint buf));
         buf <- (buf + (W64.of_int 8));
         t <- (t `^` st.[(W64.to_uint at)]);
         st.[(W64.to_uint at)] <- t;
@@ -615,7 +595,7 @@ module M = {
     while ((i \ult (W64.of_int (lEN %/ 8)))) {
       t <- st.[(W64.to_uint i)];
       i <- (i + (W64.of_int 1));
-      Glob.mem <- (storeW64 Glob.mem (W64.to_uint (buf + (W64.of_int 0))) t);
+      Glob.mem <- (storeW64 Glob.mem (W64.to_uint buf) t);
       buf <- (buf + (W64.of_int 8));
     }
     if ((0 < (lEN %% 8))) {
